Very unhappy with how this is going :(

Bytestring/Basic.lean
@@ -1,8 +1,6 @@
+import Bytestring.Bootstrap.Basic
 import Bytestring.ByteArray
 import Bytestring.Decode
-
-def List.utf8Encode (l : List Char) : ByteArray :=
-  l.flatMap String.utf8EncodeChar |>.toByteArray
 
 @[simp]
 theorem List.utf8Encode_nil : List.utf8Encode [] = ByteArray.empty := by simp [utf8Encode]
@@ -33,9 +31,6 @@ theorem utf8DecodeChar?_utf8Encode_cons {l : List Char} {c : Char} :
     utf8DecodeChar? (c::l).utf8Encode 0 = some c := by
   rw [List.utf8Encode, List.flatMap_cons, List.toByteArray_append,
     utf8DecodeChar?_utf8EncodeChar_append]
-
-structure IsValidUtf8 (b : ByteArray) : Prop where
-  exists_model : ∃ m, b = List.utf8Encode m
 
 theorem isValidUtf8_utf8Encode {l : List Char} : IsValidUtf8 l.utf8Encode where
   exists_model := ⟨l, rfl⟩
@@ -118,11 +113,6 @@ theorem ByteArray.isSome_utf8Decode?_iff {b : ByteArray} :
     b.utf8Decode?.isSome ↔ IsValidUtf8 b := by
   rw [utf8Decode?, isSome_utf8Decode?go_iff, extract_zero_size]
 
-@[ext]
-structure ByteString where
-  bytes : ByteArray
-  isValidUtf8 : IsValidUtf8 bytes
-
 def ByteString.empty : ByteString where
   bytes := ByteArray.empty
   isValidUtf8 := isValidUtf8_empty
@@ -130,28 +120,15 @@ def ByteString.empty : ByteString where
 @[simp]
 theorem ByteString.bytes_empty : ByteString.empty.bytes = ByteArray.empty := rfl
 
-def ByteString.utf8Size (s : ByteString) : Nat :=
-  s.bytes.size
-
-@[simp]
-theorem ByteString.size_bytes {s : ByteString} : s.bytes.size = s.utf8Size := rfl
-
-@[simp]
-theorem ByteString.utf8Size_empty : ByteString.empty.utf8Size = 0 := by
-  simp [← ByteString.size_bytes]
-
-@[simp]
-theorem ByteString.utf8Size_eq_zero_iff {s : ByteString} : s.utf8Size = 0 ↔ s = ByteString.empty := by
-  refine ⟨fun h => ?_, fun h => h ▸ ByteString.utf8Size_empty⟩
-  ext1
-  simp [← ByteArray.size_eq_zero_iff, h]
+-- @[simp]
+-- theorem ByteString.utf8Size_eq_zero_iff {s : ByteString} : s.utf8Size = 0 ↔ s = ByteString.empty := by
+--   refine ⟨fun h => ?_, fun h => h ▸ ByteString.utf8Size_empty⟩
+--   ext1
+--   simp [← ByteArray.size_eq_zero_iff, h]
 
 def ByteString.append (s t : ByteString) : ByteString where
   bytes := s.bytes ++ t.bytes
   isValidUtf8 := s.isValidUtf8.append t.isValidUtf8
-
-def ByteString.utf8ByteAt (s : ByteString) (byteIdx : Nat) (h : byteIdx < s.utf8Size) : UInt8 :=
-  s.bytes[byteIdx]
 
 instance : Append ByteString where
   append s t := s.append t
@@ -159,10 +136,6 @@ instance : Append ByteString where
 @[simp]
 theorem ByteString.bytes_append {s t : ByteString} : (s ++ t).bytes = s.bytes ++ t.bytes := by
   rfl
-
-@[simp]
-theorem ByteString.utf8Size_append {s t : ByteString} : (s ++ t).utf8Size = s.utf8Size + t.utf8Size := by
-  simp [← size_bytes]
 
 @[simp]
 theorem ByteString.empty_append {s : ByteString} : ByteString.empty ++ s = s := by
@@ -257,6 +230,9 @@ theorem ByteString.toByteString_data {b : ByteString} : b.data.toByteString = b 
 theorem List.toByteString_injective {l₁ l₂ : List Char} (h : l₁.toByteString = l₂.toByteString) : l₁ = l₂ := by
   simpa using congrArg ByteString.data h
 
+theorem ByteString.data_injective {s₁ s₂ : ByteString} (h : s₁.data = s₂.data) : s₁ = s₂ := by
+  simpa using congrArg List.toByteString h
+
 @[simp]
 theorem ByteString.data_append {l₁ l₂ : ByteString} : (l₁ ++ l₂).data = l₁.data ++ l₂.data := by
   apply List.toByteString_injective
@@ -266,43 +242,102 @@ theorem ByteString.data_append {l₁ l₂ : ByteString} : (l₁ ++ l₂).data = 
 theorem ByteString.utf8encode_data {b : ByteString} : b.data.utf8Encode = b.bytes :=
   congrArg ByteString.bytes (ByteString.toByteString_data (b := b))
 
-structure ByteString.ValidPos (s : ByteString) (byteIdx : Nat) : Prop where
-  exists_prefix : ∃ t₁ t₂ : ByteString, s = t₁ ++ t₂ ∧ byteIdx = t₁.utf8Size
+attribute [ext] ByteString.ByteOffset
+
+instance : OfNat ByteString.ByteOffset 0 where
+  ofNat := ⟨0⟩
+
+@[simp]
+theorem ByteString.ByteOffset.numBytes_zero : (0 : ByteOffset).numBytes = 0 := rfl
 
 @[simp, grind]
-theorem ByteString.validPos_zero {s : ByteString} : s.ValidPos 0 where
-  exists_prefix := ⟨ByteString.empty, s, by simp, by simp⟩
+theorem ByteString.validOffset_zero {s : ByteString} : s.ValidOffset 0 where
+  le_utf8Size := by simp [ByteOffset.le_iff_numBytes_le]
+  isValidUtf8 := by simp
+
+@[simp]
+theorem ByteString.utf8Size_empty : ByteString.empty.utf8Size = 0 := rfl
+
+def ByteString.Pos.toString {s : ByteString} (pos : s.Pos) : ByteString where
+  bytes := s.bytes.extract 0 pos.1.numBytes
+  isValidUtf8 := pos.2.2
+
+@[simp]
+theorem ByteString.Pos.bytes_toString {s : ByteString} {pos : s.Pos} :
+    pos.toString.bytes = s.bytes.extract 0 pos.1.numBytes := rfl
+
+def ByteString.Pos.idx {s : ByteString} (pos : s.Pos) : Nat :=
+  pos.toString.length
+
+theorem ByteString.extract_bytes_of_isPrefix (s : ByteString) (l : List Char) (hl : l <+: s.data) :
+    s.bytes.extract 0 l.utf8Encode.size = l.utf8Encode := by
+  obtain ⟨k, hk⟩ := hl
+  rw [← toByteString_data (b := s), List.bytes_toByteString, ← hk, List.utf8Encode_append,
+    ByteArray.extract_append_eq_left rfl]
+
+theorem ByteString.Pos.utf8Size_toString {s : ByteString} (pos : s.Pos) :
+    pos.toString.utf8Size = pos.offset := sorry
+
+theorem ByteString.Pos.data_toString {s : ByteString} (pos : s.Pos) :
+    pos.toString.data = s.data.take pos.idx := by
+
+  apply List.toByteString_injective
+  ext1
+  simp only [toByteString_data, bytes_toString, List.bytes_toByteString]
+  conv => rhs; rw [← ByteString.extract_bytes_of_isPrefix s (s.data.take _) (List.take_prefix _ _)]
+  congr 1
+
+  sorry
+
+
+theorem ByteString.Pos.idx_le_length {s : ByteString} (pos : s.Pos) : pos.idx ≤ s.length := by
+  sorry
+
+theorem List.IsPrefix.flatMap {l₁ l₂ : List α} {f : α → List β} (h : l₁ <+: l₂) : l₁.flatMap f <+: l₂.flatMap f := by
+  obtain ⟨k, rfl⟩ := h
+  simp
+
+theorem List.IsPrefix.utf8Size_toByteString_le {l₁ l₂ : List Char} (h : l₁ <+: l₂) : l₁.toByteString.utf8Size ≤ l₂.toByteString.utf8Size := by
+  simp [toByteString, ByteString.utf8Size, ByteString.ByteOffset.le_iff_numBytes_le]
+  simp only [utf8Encode, size_toByteArray]
+  exact h.flatMap.length_le
+
+-- TODO: this implementation is inefficient, the alternative is to call `Pos.next` `n` times
+def ByteString.nthPos (s : ByteString) (n : Nat) (_hn : n ≤ s.length) : s.Pos where
+  offset := (s.data.take n).toByteString.utf8Size
+  validOffset := {
+    le_utf8Size := by
+      conv => rhs; rw [← toByteString_data (b := s)]
+      apply List.IsPrefix.utf8Size_toByteString_le
+      exact List.take_prefix n s.data
+    isValidUtf8 := by
+      simp only [numBytes_utf8Size, List.bytes_toByteString]
+      rw [ByteString.extract_bytes_of_isPrefix _ _ (List.take_prefix n s.data)]
+      exact isValidUtf8_utf8Encode
+  }
+
+theorem ByteString.IsValidOffset.isValidUtf8' (s : ByteString) (off : ByteOffset) :
+    IsValidUtf8 (s.bytes.extract off.numBytes s.bytes.size) := sorry
 
 @[simp, grind]
-theorem ByteString.validPos_empty {byteIdx : Nat} :
-    ByteString.empty.ValidPos byteIdx ↔ byteIdx = 0 := by
+theorem ByteString.validOffset_empty {offset : ByteOffset} :
+    ByteString.empty.ValidOffset offset ↔ offset = 0 := by
   refine ⟨?_, ?_⟩
-  · rintro ⟨t₁, t₂, ht, rfl⟩
-    have := congrArg ByteString.utf8Size ht
-    simp only [utf8Size_empty, utf8Size_append] at this
+  · rintro ⟨h₁, h₂⟩
+    simp [ByteOffset.le_iff_numBytes_le] at h₁
+    ext
     omega
   · rintro rfl
     simp
 
-theorem List.validPos_toByteString {l : List Char} {byteIdx : Nat} :
-    l.toByteString.ValidPos byteIdx ↔ ∃ i, byteIdx = (l.take i).toByteString.utf8Size := by
-  refine ⟨?_, ?_⟩
-  · rintro ⟨⟨t₁, t₂, ht, rfl⟩⟩
-    refine ⟨t₁.length, ?_⟩
-    have := congrArg ByteString.data ht
-    simp at this
-    subst this
-    simp [← ByteString.size_toCharArray]
-  · rintro ⟨i, rfl⟩
-    refine ⟨⟨(l.take i).toByteString, (l.drop i).toByteString, ?_, rfl⟩⟩
-    simp [← List.toByteString_append]
+theorem List.validOffset_toByteString {l : List Char} {offset : ByteString.ByteOffset} :
+    l.toByteString.ValidOffset offset ↔ ∃ i, offset = (l.take i).toByteString.utf8Size := by
+  sorry
 
 @[simp, grind]
-theorem ByteString.validPos_utf8size {s : ByteString} : s.ValidPos s.utf8Size where
-  exists_prefix := ⟨s, ByteString.empty, by simp, by simp⟩
-
--- theorem ByteString.validPos_iff_isValidUtf8 {s : ByteString} {byteIdx : Nat} (hb : byteIdx ≤ s.utf8Size) :
---     s.ValidPos byteIdx ↔ IsValidUtf8 (s.bytes.extract 0 byteIdx) := sorry
+theorem ByteString.validOffset_utf8size {s : ByteString} : s.ValidOffset s.utf8Size where
+  le_utf8Size := Nat.le_refl _
+  isValidUtf8 := by simp [s.isValidUtf8]
 
 def UInt8.IsUtf8FirstByte (c : UInt8) : Prop :=
   c &&& 0x80 = 0 ∨ c &&& 0xe0 = 0xc0 ∨ c &&& 0xf0 = 0xe0 ∨ c &&& 0xf8 = 0xf0
@@ -322,9 +357,47 @@ def ByteString.push (b : ByteString) (c : Char) : ByteString where
 @[simp]
 theorem ByteString.bytes_push {s : ByteString} {c : Char} : (s.push c).bytes = s.bytes ++ [c].utf8Encode := rfl
 
+instance : Add ByteString.ByteOffset where
+  add a b := ⟨a.numBytes + b.numBytes⟩
+
+instance : Sub ByteString.ByteOffset where
+  sub a b := ⟨a.numBytes - b.numBytes⟩
+
+instance : LT ByteString.ByteOffset where
+  lt a b := a.numBytes < b.numBytes
+
 @[simp]
-theorem ByteString.utf8Size_push {s : ByteString} {c : Char} : (s.push c).utf8Size = s.utf8Size + c.utf8Size := by
-  simp [← size_bytes, List.utf8Encode_singleton]
+theorem ByteString.ByteOffset.numBytes_add {a b : ByteString.ByteOffset} :
+    (a + b).numBytes = a.numBytes + b.numBytes := rfl
+
+@[simp]
+theorem ByteString.ByteOffset.numBytes_sub {a b : ByteString.ByteOffset} :
+    (a - b).numBytes = a.numBytes - b.numBytes := rfl
+
+theorem ByteString.ByteOffset.lt_iff_numBytes_lt {a b : ByteString.ByteOffset} :
+    a < b ↔ a.numBytes < b.numBytes := Iff.rfl
+
+def ByteString.utf8ByteAt (s : ByteString) (off : ByteString.ByteOffset) (h : off < s.utf8Size) : UInt8 :=
+  s.bytes[off.numBytes]
+
+@[simp]
+theorem ByteString.utf8Size_append {s t : ByteString} : (s ++ t).utf8Size = s.utf8Size + t.utf8Size := by
+  ext
+  simp
+
+def Char.utf8Size' (c : Char) : ByteString.ByteOffset :=
+  ⟨c.utf8Size⟩
+
+@[simp]
+theorem Char.numBytes_utf8Size' {c : Char} : c.utf8Size'.numBytes = c.utf8Size := rfl
+
+theorem Char.utf8Size'_pos {c : Char} : 0 < c.utf8Size' := by
+  simp [ByteString.ByteOffset.lt_iff_numBytes_lt, Char.utf8Size_pos]
+
+@[simp]
+theorem ByteString.utf8Size_push {s : ByteString} {c : Char} : (s.push c).utf8Size = s.utf8Size + c.utf8Size' := by
+  ext
+  simp [List.utf8Encode_singleton]
 
 @[simp]
 theorem ByteString.append_toByteString_singleton {s : ByteString} {c : Char} :
@@ -340,7 +413,8 @@ theorem ByteString.bytes_singleton {c : Char} : (ByteString.singleton c).bytes =
   simp [singleton]
 
 @[simp, grind]
-theorem ByteString.utf8size_singleton {c : Char} : (ByteString.singleton c).utf8Size = c.utf8Size := by
+theorem ByteString.utf8size_singleton {c : Char} : (ByteString.singleton c).utf8Size = c.utf8Size' := by
+  ext
   simp [singleton]
 
 theorem ByteString.singleton_eq_toByteString {c : Char} : ByteString.singleton c = [c].toByteString := by
@@ -449,9 +523,9 @@ theorem isUtf8FirstByte_getElem_utf8Encode_singleton {c : Char} {i : Nat} {hi : 
     UInt8.IsUtf8FirstByte [c].utf8Encode[i] ↔ i = 0 := by
   simp [List.utf8Encode_singleton, isUtf8FirstByte_getElem_utf8EncodeChar]
 
-theorem ByteString.validPos_singleton {c : Char} {byteIdx : Nat} :
-    (ByteString.singleton c).ValidPos byteIdx ↔ byteIdx = 0 ∨ byteIdx = c.utf8Size := by
-  rw [singleton_eq_toByteString, List.validPos_toByteString]
+theorem ByteString.validOffset_singleton {c : Char} {off : ByteString.ByteOffset} :
+    (ByteString.singleton c).ValidOffset off ↔ off = 0 ∨ off = c.utf8Size' := by
+  rw [singleton_eq_toByteString, List.validOffset_toByteString]
   refine ⟨?_, ?_⟩
   · rintro ⟨i, rfl⟩
     obtain ⟨rfl, hi⟩ : i = 0 ∨ 1 ≤ i := by omega
@@ -471,56 +545,69 @@ theorem ByteString.append_singleton {s : ByteString} {c : Char} :
 theorem List.take_eq_take_min {l : List α} {i : Nat} : l.take i = l.take (min i l.length) := by
   simp [List.take_eq_take_iff]
 
-theorem ByteString.validPos_append {s t : ByteString} {byteIdx : Nat} :
-    (s ++ t).ValidPos byteIdx ↔ s.ValidPos byteIdx ∨ (s.utf8Size ≤ byteIdx ∧ t.ValidPos (byteIdx - s.utf8Size)) := by
+theorem ByteString.validOffset_append {s t : ByteString} {off : ByteString.ByteOffset} :
+    (s ++ t).ValidOffset off ↔ s.ValidOffset off ∨ (s.utf8Size ≤ off ∧ t.ValidOffset (off - s.utf8Size)) := by
   obtain ⟨s, rfl⟩ := exists_eq_toByteString s
   obtain ⟨t, rfl⟩ := exists_eq_toByteString t
-  rw [← List.toByteString_append, List.validPos_toByteString, List.validPos_toByteString, List.validPos_toByteString]
+  rw [← List.toByteString_append, List.validOffset_toByteString, List.validOffset_toByteString, List.validOffset_toByteString]
   refine ⟨?_, ?_⟩
   · rintro ⟨j, rfl⟩
     by_cases h : j ≤ s.length
     · exact Or.inl ⟨j, by simp [List.take_append_of_le_length h]⟩
     · refine Or.inr ⟨?_, ⟨j - s.length, ?_⟩⟩ <;>
-        simp [List.take_append, List.take_of_length_le (i := j) (l := s) (by omega)]
+        simp [List.take_append, List.take_of_length_le (i := j) (l := s) (by omega), ByteString.ByteOffset.le_iff_numBytes_le,
+          ByteString.ByteOffset.ext_iff]
   · rintro (⟨j, rfl⟩|⟨h, ⟨j, hj⟩⟩)
     · refine ⟨min j s.length, ?_⟩
       rw [List.take_append_of_le_length (Nat.min_le_right ..), ← List.take_eq_take_min]
     · refine ⟨s.length + j, ?_⟩
-      simp [List.take_append, List.take_of_length_le (i := s.length + j) (l := s) (by omega)]
+      simp only [ByteOffset.ext_iff, ByteOffset.numBytes_sub, numBytes_utf8Size,
+        List.bytes_toByteString, ByteOffset.le_iff_numBytes_le] at hj h
+      simp [List.take_append, List.take_of_length_le (i := s.length + j) (l := s) (by omega), ByteString.ByteOffset.ext_iff]
       omega
 
-theorem ByteString.validPos_push {s : ByteString} {c : Char} {byteIdx : Nat} :
-    (s.push c).ValidPos byteIdx ↔ s.ValidPos byteIdx ∨ byteIdx = (s.push c).utf8Size := by
-  rw [← append_singleton, validPos_append, validPos_singleton, utf8Size_append]
-  grind
+theorem ByteString.validOffset_push {s : ByteString} {c : Char} {off : ByteString.ByteOffset} :
+    (s.push c).ValidOffset off ↔ s.ValidOffset off ∨ off = (s.push c).utf8Size := by
+  rw [← append_singleton, validOffset_append, validOffset_singleton, utf8Size_append]
+  simp [ByteString.ByteOffset.ext_iff, ByteString.ByteOffset.le_iff_numBytes_le, ByteString.ByteOffset.numBytes_sub]
+  refine ⟨?_, ?_⟩
+  · rintro (h|⟨h₁,(h₂|h₂)⟩)
+    · grind
+    · suffices off = s.utf8Size by grind
+      simp [ByteString.ByteOffset.ext_iff]
+      omega
+    · grind
+  · grind
 
 theorem ByteString.push_induction (s : ByteString) (motive : ByteString → Prop) (empty : motive ByteString.empty)
     (push : ∀ b c, motive b → motive (b.push c)) : motive s := sorry
 
-theorem ByteString.validPos_iff_isUtf8FirstByte (s : ByteString) (byteIdx : Nat) :
-    s.ValidPos byteIdx ↔
-      (byteIdx = s.utf8Size ∨ (∃ (h : byteIdx < s.utf8Size), UInt8.IsUtf8FirstByte (s.utf8ByteAt byteIdx h))) := by
+theorem ByteString.validPos_iff_isUtf8FirstByte (s : ByteString) (off : ByteString.ByteOffset) :
+    s.ValidOffset off ↔
+      (off = s.utf8Size ∨ (∃ (h : off < s.utf8Size), UInt8.IsUtf8FirstByte (s.utf8ByteAt off h))) := by
   induction s using ByteString.push_induction with
-  | empty => simp
+  | empty => simp [ByteString.ByteOffset.lt_iff_numBytes_lt]
   | push s c ih =>
-    rw [validPos_push, ih]
+    rw [validOffset_push, ih]
     refine ⟨?_, ?_⟩
     · rintro ((rfl|⟨h, hb⟩)|h)
-      · refine Or.inr ⟨by simp [Char.utf8Size_pos], ?_⟩
-        simp only [utf8ByteAt, bytes_push, ← size_bytes]
+      · refine Or.inr ⟨by simp [ByteString.ByteOffset.lt_iff_numBytes_lt, Char.utf8Size_pos], ?_⟩
+        simp only [utf8ByteAt, bytes_push, numBytes_utf8Size]
         rw [ByteArray.getElem_append_right (Nat.le_refl _)]
         simp [isUtf8FirstByte_getElem_utf8Encode_singleton]
-      · refine Or.inr ⟨by simp; omega, ?_⟩
+      · refine Or.inr ⟨by simp [ByteString.ByteOffset.lt_iff_numBytes_lt] at h; simp [ByteString.ByteOffset.lt_iff_numBytes_lt]; omega, ?_⟩
         simp only [utf8ByteAt, bytes_push]
         rwa [ByteArray.getElem_append_left, ← utf8ByteAt]
       · exact Or.inl h
     · rintro (h|⟨h, hb⟩)
       · exact Or.inr h
       · simp only [utf8ByteAt, bytes_push] at hb
-        by_cases h' : byteIdx < s.utf8Size
+        by_cases h' : off < s.utf8Size
         · refine Or.inl (Or.inr ⟨h', ?_⟩)
           rwa [ByteArray.getElem_append_left h', ← utf8ByteAt] at hb
         · refine Or.inl (Or.inl ?_)
-          rw [ByteArray.getElem_append_right (by simp; omega)] at hb
+          rw [ByteArray.getElem_append_right (by simp [ByteString.ByteOffset.lt_iff_numBytes_lt] at h'; omega)] at hb
           simp [isUtf8FirstByte_getElem_utf8Encode_singleton] at hb
+          ext
+          simp [ByteString.ByteOffset.lt_iff_numBytes_lt] at ⊢ h'
           omega
