Bytestring/Bootstrap/Basic.lean
@@ -1,0 +1,58 @@
+import Bytestring.Bootstrap.ByteArray
+
+def List.utf8Encode (l : List Char) : ByteArray :=
+  l.flatMap String.utf8EncodeChar |>.toByteArray
+
+structure IsValidUtf8 (b : ByteArray) : Prop where
+  exists_model : ∃ m, b = List.utf8Encode m
+
+@[simp]
+theorem IsValidUtf8.empty : IsValidUtf8 ByteArray.empty where
+  exists_model := ⟨[], rfl⟩
+
+@[ext]
+structure ByteString where
+  bytes : ByteArray
+  isValidUtf8 : IsValidUtf8 bytes
+
+structure ByteString.ByteOffset where
+  numBytes : Nat
+
+def ByteString.utf8Size (s : ByteString) : ByteString.ByteOffset :=
+  ⟨s.bytes.size⟩
+
+instance : LE ByteString.ByteOffset where
+  le a b := a.numBytes ≤ b.numBytes
+
+theorem ByteString.ByteOffset.le_iff_numBytes_le {a b : ByteString.ByteOffset} :
+    a ≤ b ↔ a.numBytes ≤ b.numBytes := Iff.rfl
+
+@[simp]
+theorem ByteString.numBytes_utf8Size (s : ByteString) :
+  s.utf8Size.numBytes = s.bytes.size := rfl
+
+structure ByteString.ValidOffset (s : ByteString) (off : ByteOffset) where
+  le_utf8Size : off ≤ s.utf8Size
+  isValidUtf8 : IsValidUtf8 (s.bytes.extract 0 off.numBytes)
+
+structure ByteString.Pos (s : ByteString) where
+  offset : ByteOffset
+  validOffset : s.ValidOffset offset
+
+def ByteString.startPos (s : ByteString) : s.Pos where
+  offset := ⟨0⟩
+  validOffset := ⟨by simp [ByteOffset.le_iff_numBytes_le], by simp⟩
+
+def ByteString.endPos (s : ByteString) : s.Pos where
+  offset := s.utf8Size
+  validOffset := ⟨by simp [ByteOffset.le_iff_numBytes_le], by simpa using s.isValidUtf8⟩
+
+structure ByteString.Slice where
+  str : ByteString
+  startInclusive : str.Pos
+  endExclusive : str.Pos
+
+def ByteString.toSlice (s : ByteString) : ByteString.Slice where
+  str := s
+  startInclusive := s.startPos
+  endExclusive := s.endPos
