Bytestring/Bootstrap/ByteArray.lean
@@ -1,0 +1,22 @@
+@[simp]
+theorem ByteArray.data_empty : ByteArray.empty.data = #[] := rfl
+
+@[simp]
+theorem ByteArray.data_extract {a : ByteArray} {b e : Nat} :
+    (a.extract b e).data = a.data.extract b e := by
+  simp [extract, copySlice]
+  grind
+
+@[simp]
+theorem ByteArray.size_data {a : ByteArray} :
+  a.data.size = a.size := rfl
+
+@[simp]
+theorem ByteArray.extract_zero_size {b : ByteArray} : b.extract 0 b.size = b := by
+  ext1
+  simp
+
+@[simp]
+theorem ByteArray.extract_same {b : ByteArray} {i : Nat} : b.extract i i = ByteArray.empty := by
+  ext1
+  simp [Nat.min_le_left]
